\documentclass[12pt, a4paper]{article}

\usepackage{algorithmic}

\begin{document}
\begin{algorithmic}
    \STATE States $q_C = [q_A, q_B, q_{EBA}, q_{EBB}, w, i, k]$\\
    \STATE $q_A \in Q_A$\\
    \STATE $q_B \in Q_B$\\
    \STATE $q_{EBA} = $ state of Eilenburg bimachine A
    \STATE $q_{EBB} = $ state of Eilenburg bimachine B
    \STATE $w \in \Gamma^* = $ intermediate word buffer\\
    \STATE $i \in |w| = $ position in $w$\\
    \STATE $k \in \dots = $ control pointer\\
    \STATE $k = 0 : $ initialising the bimachines\\
    \STATE $k = 1 : $ simulating A and B\\
    \STATE $k = 2 : $ look one to the right to backtrack bimachine EBB\\
    \STATE $k = 4 : $ look one to the left to backtrack bimachine EBA\\


    \STATE Initial state: $q_{C0} = [q_{A0}, q_{B0}, q_{EBA0}, q_{EBB0}, \epsilon, 0, 1]$
    \STATE $q_{EBA0} = ([], [])$
    \STATE $q_{EBB0} = ([])$
    \STATE $\delta_A(q_{A0}, <) \gets (q_A', d, <w)$ where $\delta_A(q_{A0}, <) = (q_A', d, w)$

    % \STATE Initialising the bimachines:
    % \STATE $\delta_C(q_{C0}, <) = (q_{C0}, +1, \epsilon)$
    % \STATE $\delta_C(q_{C0}, \sigma) = (q_{C0}, +1, \epsilon)$
    % \STATE $\delta_C(q_{C0}, >) = ([q_{A0}, q_{B0}, q_{EBA0}, q_{EBB}', \epsilon, 0, 0], -1, \epsilon)$ where $\delta_{EBB}(q_{EBB0}, >) = q_{EBB}'$
    % \STATE $\delta_C([q_{A0}, q_{B0}, q_{EBA0}, q_{EBB}, \epsilon, 0, 0], \sigma) = ([q_{A0}, q_{B0}, q_{EBA0}, q_{EBB}', \epsilon, 0, 0], -1, \epsilon)$ where $\delta_{EBB}(q_{EBB},\sigma) = q_{EBB}'$
    % \STATE $\delta_C([q_{A0}, q_{B0}, q_{EBA0}, q_{EBB}, \epsilon, 0, 0], <) = ([q_{A0}, q_{B0}, q_{EBA0}, q_{EBB}, \epsilon, 0, 1], 0, \epsilon)$
    

    \STATE Accepting condition:
    \STATE $\delta_C([q_A, q_{Baccept}, q_{EBA}, q_{EBB}, w, i, 1], \sigma) = (q_{Caccept}, 0, \epsilon)$


    \STATE Simulating transducer A to get the next w for transducer B to use:
    \STATE $\delta_C([q_A, q_B, q_{EBA}, q_{EBB}, w, |w|, 1], \sigma) = $\\
        \IF{$\delta_A(q_A, \sigma) = (a_Aaccept, 0, \epsilon)$}
            \STATE $([q_Aaccept, q_B, q_{EBA}, q_{EBB}, >, 0, 1], 0, \epsilon)$
        \ELSIF{$\delta_A(q_A, \sigma) = (q_A', 0, u)$}
            \STATE $([q_A', q_B, q_{EBA}, q_{EBB}, u, 0, 1], 0, \epsilon)$
        \ELSIF{$\delta_A(q_A, \sigma) = (q_A', +1, u)$ AND $\sigma \neq >$}
            \STATE $([q_A', q_B, q_{EBA}', q_{EBB}, u, 0, 2], +1, \epsilon)$ where $\delta_{EBA}(q_{EBA}, \sigma) = q_{EBA}'$
        \ELSIF{$\delta_A(q_A, \sigma) = (q_A', -1, u)$ AND $\sigma \neq <$}
            \STATE $([q_A', q_B, q_{EBA}, q_{EBB}', u, 0, 4], -1, \epsilon)$ where $\delta_{EBB}(q_{EBB}, \sigma) = q_{EBB}'$
        \ENDIF
    
    \STATE $\delta_C([q_A, q_B, q_{EBA}, q_{EBB}, w, 0, 2], >) = ([q_A, q_B, q_{EBA}, q_{EBB0}, w, 0, 1], 0, \epsilon)$
    \STATE $\delta_C([q_A, q_B, q_{EBA}, q_{EBB}, w, 0, 2], \sigma) = ([q_A, q_B, q_{EBA}, q_{EBB}, w, 0, 3], +1, \epsilon)$
    \STATE $\delta_C([q_A, q_B, q_{EBA}, q_{EBB}, w, 0, 3], \sigma) = ([q_A, q_B, q_{EBA}, q_{EBB}', w, 0, 1], -1, \epsilon)$ where $q_{EBB}'$ can be derived from the available information

    \STATE $\delta_C([q_A, q_B, q_{EBA}, q_{EBB}, w, 0, 4], <) = ([q_A, q_B, q_{EBA0}, q_{EBB}, w, 0, 1], 0, \epsilon)$
    \STATE $\delta_C([q_A, q_B, q_{EBA}, q_{EBB}, w, 0, 4], \sigma) = ([q_A, q_B, q_{EBA}, q_{EBB}, w, 0, 5], -1, \epsilon)$
    \STATE $\delta_C([q_A, q_B, q_{EBA}, q_{EBB}, w, 0, 5], \sigma) = ([q_A, q_B, q_{EBA}', q_{EBB}, w, 0, 1], +1, \epsilon)$ where $q_{EBA}'$ can be derived from the available information


    \STATE Simulating transducer B on w:
    \STATE $\delta_C([q_A, q_B, q_{EBA}, q_{EBB}, w, i, 1], \sigma) = $
        \IF{$\delta_B(q_B, w[i]) = (q_B', 0, u)$}
            \STATE $([q_A, q_B', q_{EBA}, q_{EBB}, w, i, 1], 0, u)$ 
        \ELSIF{$\delta_B(q_B, w[i]) = (q_B', +1, u)$ AND $w[i] \neq >$}
            \STATE $([q_A, q_B', q_{EBA}, q_{EBB}, w, i+1, 1], 0, u)$ 
        \ELSIF{$\delta_B(q_B, w[i]) = (q_B', -1, u)$ AND $w[i] \neq <$}
            \STATE $([q_A, q_B', q_{EBA}, q_{EBB}, w, i-1, 1], 0, u)$ 
        \ENDIF

    \STATE Backtrack transducer A if transducer B needs to go left out of w:
    \STATE $\gamma(q_{EBA}, q_{EBB}, \sigma) = \alpha$
    \STATE $\delta_C([q_A, q_B, q_{EBA}, q_{EBB}, w, -1, 1], \sigma) = $\\
    \IF{$\alpha(q_A) = 0$}
        \STATE $([q_A', q_B, q_{EBA}, q_{EBB}, u, |u| - 1, 1], 0, \epsilon)$ where $\delta_A(q_A', \sigma) = (q_A, 0, u)$
    \ELSIF{$\alpha(q_A) = +1$}
        \STATE $([q_A, q_B, q_{EBA}', q_{EBB}, w, -1, 6], +1, \epsilon)$ where $\delta_{EBA}(q_{EBA}, \sigma) = q_{EBA}'$
    \ELSIF{$\alpha(q_A) = -1$}
        \STATE $([q_A, q_B, q_{EBA}, q_{EBB}', w, -1, 8], -1, \epsilon)$ where $\delta_{EBB}(q_{EBB}, \sigma) = q_{EBB}'$
    \ENDIF

    \STATE $\delta_C([q_A, q_B, q_{EBA}, q_{EBB}, w, -1, 6], \sigma) = ([q_A, q_B, q_{EBA}, q_{EBB}, w, -1, 7], +1, \epsilon)$
    \STATE $\delta_C([q_A, q_B, q_{EBA}, q_{EBB}, w, -1, 7], \sigma) = ([q_A', q_B, q_{EBA}, q_{EBB}', u, |u|-1, 1], -1, \epsilon)$ where $q_{EBB}'$ can be derived from the available information and $\delta_A(q_A', \sigma) = (q_A, -1, u)$

    \STATE $\delta_C([q_A, q_B, q_{EBA}, q_{EBB}, w, -1, 8], \sigma) = ([q_A, q_B, q_{EBA}, q_{EBB}, w, 0, 8], -1, \epsilon)$
    \STATE $\delta_C([q_A, q_B, q_{EBA}, q_{EBB}, w, -1, 9], \sigma) = ([q_A', q_B, q_{EBA}', q_{EBB}, u, |u|-1, 1], +1, \epsilon)$ where $q_{EBA}'$ can be derived from the available information and $\delta_A(q_A', \sigma) = (q_A, +1, u)$


\end{algorithmic}
\pagebreak



\begin{algorithmic}
    \STATE $\delta_C([q_A, q_B, \alpha_0 \alpha_1 \alpha_2, w, |w|, j, 1], \sigma) =$\\
        \IF{$\alpha_j(q_A) = (q_A', 0, u)$}
            \STATE $([q_A', q_B, \alpha_0 \alpha_1 \alpha_2, u, 0, j, 1], 0, \epsilon)$\\
        \ELSIF{$\alpha_j(q_A) = (q_A', +1, u)$}
            \IF{$(j \in \{0,1\})$}
                \STATE $([q_A', q_B, \alpha_0 \alpha_1 \alpha_2, u, 0, j+1, 1], 0, \epsilon)$\\
            \ELSIF{$(j = 2)$}
                \STATE $([q_A', q_B, \alpha_0 \alpha_1 \alpha_2, u, 0, 2, 2], +1, \epsilon)$\\
            \ENDIF
        \ELSIF{$\alpha_j(q_A) = (q_A', -1, u)$}
            \IF{$(j \in \{1, 2\})$}
                \STATE $([q_A', q_B, \alpha_0 \alpha_1 \alpha_2, u, 0, j-1, 1], 0, \epsilon)$\\
            \ELSIF{$(j = 0)$}
                \STATE $([q_A', q_B, \alpha_0 \alpha_1 \alpha_2, u, 0, 0, 4], -1, \epsilon)$\\
            \ENDIF
        \ENDIF
    
    \STATE $\delta_C([q_A, q_B, \alpha_0 \alpha_1 \alpha_2, w, 0, 2, 2], \sigma) = ([q_A, q_B, \alpha_0 \alpha_1 \alpha_2, w, 0, 2, 3], +1, \epsilon)$\\
    \STATE $\delta_C([q_A, q_B, \alpha_0 \alpha_1 \alpha_2, w, 0, 2, 3], \sigma) = ([q_A, q_B, \alpha_0' \alpha_1' \alpha_2', w, 0, 2, 1], -1, \epsilon)$\\s.t. $\alpha_0' = \alpha_1, \alpha_1' = \alpha_2, \alpha_2' = G(\sigma)$
    
    \STATE $\delta_C([q_A, q_B, \alpha_0 \alpha_1 \alpha_2, w, 0, 0, 4], \sigma) = ([q_A, q_B, \alpha_0 \alpha_1 \alpha_2, w, 0, 0, 5], -1, \epsilon)$\\
    \STATE $\delta_C([q_A, q_B, \alpha_0 \alpha_1 \alpha_2, w, 0, 0, 5], \sigma) = ([q_A, q_B, \alpha_0' \alpha_1' \alpha_2', w, 0, 0, 1], +1, \epsilon)$\\s.t. $\alpha_2' = \alpha_1, \alpha_1' = \alpha_0, \alpha_0' = G(\sigma)$



    \STATE $\delta_C([q_A, q_B, \alpha_0 \alpha_1 \alpha_2, w, -1, j, 1], \sigma) =$\\
        \IF{$F(\alpha_0 \alpha_1 \alpha_2, j, q_A) \in \{0, 1, 2\}$}
            \STATE ($[q_A', q_B, \alpha_0 \alpha_1 \alpha_2, u, |u|-1, F(\alpha_0 \alpha_1 \alpha_2, j, q_A), 1], 0, \epsilon)$\\s.t. $\alpha_{F(\alpha_0 \alpha_1 \alpha_2, j, q_A)}(q_A') = (q_A, d, u)$
        \ELSIF{$j = 2$}
            \STATE $([q_A, q_B, \alpha_0 \alpha_1 \alpha_2, w, -1, 2, 6], +1, \epsilon)$
        \ELSIF{$j = 0$}
            \STATE $([q_A, q_B, \alpha_0 \alpha_1 \alpha_2, w, -1, 2, 8], -1, \epsilon)$
        \ENDIF

    \STATE $\delta_C([q_A, q_B, \alpha_0 \alpha_1 \alpha_2, w, -1, 2, 6], \sigma) = ([q_A, q_B, \alpha_0 \alpha_1 \alpha_2, w, -1, 2, 7], +1, \epsilon)$
    \STATE $\delta_C([q_A, q_B, \alpha_0 \alpha_1 \alpha_2, w, -1, 2, 7], \sigma) = ([q_A', q_B, \alpha_0' \alpha_1' \alpha_2', u, |u|-1, 2, 1], -1, \epsilon)$\\s.t. $\alpha_0' = \alpha_1, \alpha_1' = \alpha_2, \alpha_2' = G(\sigma), \alpha_2'(q_A') = (q_A, -1, u)$

    \STATE $\delta_C([q_A, q_B, \alpha_0 \alpha_1 \alpha_2, w, -1, 2, 8], \sigma) = ([q_A, q_B, \alpha_0 \alpha_1 \alpha_2, w, -1, 2, 9], -1, \epsilon)$
    \STATE $\delta_C([q_A, q_B, \alpha_0 \alpha_1 \alpha_2, w, -1, 2, 9], \sigma) = ([q_A', q_B, \alpha_0' \alpha_1' \alpha_2', u, |u|-1, 2, 1], +1, \epsilon)$\\s.t. $\alpha_2' = \alpha_1, \alpha_1' = \alpha_0, \alpha_0' = G(\sigma), \alpha_0'(q_A') = (q_A, -1, u)$

    \STATE $\delta_C([q_A, q_B, \alpha_0 \alpha_1 \alpha_2, w, i, j, 1], \sigma) = ([q_A, q_B', \alpha_0 \alpha_1 \alpha_2, w, i+d, j, 1], 0, u)$\\s.t. $(q_B', d, u) = \delta_B(q_B, w[i])$
\end{algorithmic}
\pagebreak
\begin{algorithmic}
    \STATE Eilenburg Bimachine Definition:
    \STATE $EB = (A, B, \Sigma, \Gamma, \gamma)$
    \STATE $A = (Q_{EBA}, \Sigma, \delta_{EBA})$ Left to right sequential
    \STATE $Q_{EBA} = (\subseteq Q_A \times Q_A, \subseteq Q_A)$ (all paths from column $i-1$ to $i-1$ while only visiting configurations $< i$, all states in layer $i-1$ that are reachable from the initial state while staying $< i$)
    \STATE $\delta_{EBA}: Q_{EBA} \times \Sigma \to Q_{EBA}$
    \STATE $B = (Q_{EBB}, \Sigma, \delta_{EBB})$ Right to left sequential
    \STATE $Q_{EBB} = (\subseteq Q_A \times Q_A)$ (all paths from column $i+1$ to $i + 1$ while only visiting configurations $> i$)
    \STATE $\delta_{EBB}: Q_{EBB} \times \Sigma \to Q_{EBB}$
    \STATE $\Sigma = $ Input alphabet
    \STATE $ \Gamma = $ Output alphabet
    \STATE $\gamma = $ Output function
    \STATE $\gamma: Q_{EBA} \times Q_{EBB} \times \Sigma \to \Gamma$
\end{algorithmic}


\end{document}